theories/Strl.v
@@ -2,37 +2,59 @@ Require Import List Uint63 PString Recdef Lia ZifyUint63.
 Open Scope uint63.
 Open Scope pstring.
 
-Definition strl := list string.
-Fixpoint slget sl i :=
+Definition strl := {x: list string | Forall (fun x => x <> "") x}.
+Fixpoint _slget sl i :=
   match sl with
   | nil => 0
   | a::t =>
       if (i <? length a)
       then get a i
-      else slget t (i - length a)
+      else _slget t (i - length a)
   end.
-Definition slcat := @app string.
-Fixpoint slsub sl i n :=
+Definition slget (sl:strl) i := _slget (proj1_sig sl) i.
+Definition _slcat := @app string.
+Definition slcat (sl1 sl2: strl) : strl.
+Proof.
+  inversion sl1. inversion sl2.
+  exists (x++x0). now apply Forall_app.
+Defined.
+Fixpoint _slsub sl i n :=
   if (n =? 0) then nil else
   match sl with
   | nil => nil
   | a::t =>
       if (i <? length a) then
         let x := sub a i n in
-        x::slsub t 0 (n - length x)
+        x::_slsub t 0 (n - length x)
       else
-        slsub t (i - length a) n
+        _slsub t (i - length a) n
   end.
-Definition sllength sl :=
-  List.fold_left add (map length sl) 0.
-
-Lemma sub_len_0:
-  forall off sl, slsub sl off 0 = nil.
-Proof. now destruct sl. Qed.
-Lemma sub_full:
-  forall sl, slsub sl 0 (sllength sl) = sl.
-Proof. induction sl. easy. simpl. unfold sllength.
-
-Import ListNotations.
-Compute (slget ["01";"2345";"6789";"012345";"6"] 17).
-Compute slget ["1"] 1.
+Definition slsub (sl: strl) (i n: int) : strl.
+Proof.
+  inversion sl. exists (_slsub x i n).
+  generalize n i. induction x; intros; simpl.
+  - now destruct eqb.
+  - destruct eqb eqn:NE; auto. apply Forall_inv_tail in H.
+    destruct ltb eqn:LT; [| now apply IHx].
+    constructor; [| now apply IHx].
+    intro S; apply (f_equal to_list) in S.
+    rewrite sub_spec in S.
+    apply (f_equal (@List.length _)) in S; cbv [to_list] in S.
+    rewrite length_firstn, length_skipn, length_map, length_seq in S.
+    simpl in S. lia.
+Defined.
+Definition _sllength sl := List.fold_left add (map length sl) 0.
+Definition sllength (sl: strl) := _sllength (proj1_sig sl).
+Definition strl_of_list (sl: list string) : strl.
+Proof.
+  exists (filter (fun x => match compare x "" with | Eq => false | _ => true end) sl).
+  apply Forall_forall. intros. apply filter_In in H as [_ H].
+  intro. now rewrite H0 in H.
+Defined.
+Definition strl_of_string (s: string) : strl.
+Proof.
+  destruct (compare s "") eqn:E. now exists nil.
+  all: exists (s::nil); constructor; try easy; intro; now rewrite H in E.
+Defined.
+Definition slsplice sl i sl2 :=
+  slcat (slcat (slsub sl 0 i) sl2) (slsub sl (i + sllength sl2) (sllength sl)).
